Completed closure proofs for instantaneous reactive designs

theories/utp_rea_designs.thy
@@ -4703,7 +4703,7 @@ subsection {* Algebraic Laws *}
 lemma assigns_srd_left_seq:
   assumes "P is NSRD"
   shows "\<langle>\<sigma>\<rangle>\<^sub>R ;; P = (\<lceil>\<sigma>\<rceil>\<^sub>S\<^sub>\<sigma> \<dagger> P)"
-  by (rdes_simp cls: assms)  
+  by (rdes_simp cls: assms)
    
 subsection {* Instantaneous Reactive Designs *}
   
@@ -4711,16 +4711,16 @@ definition ISRD1 :: "('s,'t::trace,'\<alpha>) hrel_rsp \<Rightarrow> ('s,'t,'\<a
 [upred_defs]: "ISRD1(P) = P \<parallel>\<^sub>R choose\<^sub>R"
 
 definition ISRD :: "('s,'t::trace,'\<alpha>) hrel_rsp \<Rightarrow> ('s,'t,'\<alpha>) hrel_rsp" where
-[upred_defs, rdes_def]: "ISRD = ISRD1 \<circ> NSRD"
+[upred_defs]: "ISRD = ISRD1 \<circ> NSRD"
 
 lemma choose_srd_par: 
   "choose\<^sub>R \<parallel>\<^sub>R choose\<^sub>R = choose\<^sub>R"
   by (rdes_eq)
 
-lemma ISRD_idem: "ISRD1(ISRD1(P)) = ISRD1(P)"
+lemma ISRD1_idem: "ISRD1(ISRD1(P)) = ISRD1(P)"
   by (rel_auto)
     
-lemma ISRD_monotonic: "P \<sqsubseteq> Q \<Longrightarrow> ISRD1(P) \<sqsubseteq> ISRD1(Q)"
+lemma ISRD1_monotonic: "P \<sqsubseteq> Q \<Longrightarrow> ISRD1(P) \<sqsubseteq> ISRD1(Q)"
   by (rel_auto)
 
 lemma ISRD1_rdes_def [rdes_def]: 
@@ -4738,11 +4738,132 @@ proof -
   thus ?thesis
     by (simp add: ISRD_def Healthy_comp assms(1))
 qed
-      
+
+lemma ISRD_rdes_intro [closure]:
+  assumes "P is RC" "Q is RR"
+  shows "\<^bold>R\<^sub>s(P \<turnstile> false \<diamondop> Q) is ISRD"
+  by (simp_all add: ISRD_intro closure assms unrest rdes)
+  
+lemma ISRD_implies_ISRD1:
+  assumes "P is ISRD"
+  shows "P is ISRD1"
+proof -
+  have "ISRD(P) is ISRD1"
+    by (simp add: ISRD_def Healthy_def ISRD1_idem)
+  thus ?thesis
+    by (simp add: assms Healthy_if)
+qed
+  
+lemma ISRD_implies_SRD: 
+  assumes "P is ISRD"
+  shows "P is SRD"
+proof -
+  have 1:"ISRD(P) = \<^bold>R\<^sub>s((\<not>\<^sub>r (\<not>\<^sub>r pre\<^sub>R P) ;; R1 true \<and> R1 true) \<turnstile> false \<diamondop> (post\<^sub>R P \<and> R1 true))"
+    by (simp add: NSRD_form ISRD1_def ISRD_def RHS_tri_design_par rdes_def unrest closure)
+  moreover have "... is SRD"
+    by (simp add: closure unrest)
+  ultimately have "ISRD(P) is SRD"
+    by (simp)
+  with assms show ?thesis
+    by (simp add: Healthy_def)
+qed
+    
+lemma RC1_RR_closed: "P is RR \<Longrightarrow> RC1(P) is RR"
+  by (simp add: RC1_def closure)
+
+lemma wpR_R2_closed [closure]:
+  "\<lbrakk> P is R2; Q is R2 \<rbrakk> \<Longrightarrow> P wp\<^sub>R Q is R2"
+  by (simp add: wpR_def closure)
+
+lemma wpR_false_RC1': "P is R2 \<Longrightarrow> RC1(P wp\<^sub>R false) = P wp\<^sub>R false"
+  by (simp add: wpR_def RC1_def closure rpred seqr_assoc)
+    
+lemma wpR_false_RC1: "P is R2 \<Longrightarrow> P wp\<^sub>R false is RC1"
+  by (simp add :Healthy_def wpR_false_RC1')
+  
+lemma wpR_false_RR:
+  "\<lbrakk> $ok \<sharp> P; $wait \<sharp> P; P is R2 \<rbrakk> \<Longrightarrow> P wp\<^sub>R false is RR"
+  by (rule RR_R2_intro, simp_all add: unrest closure)
+
+lemma wpR_false_RC:
+  "\<lbrakk> $ok \<sharp> P; $wait \<sharp> P; P is R2 \<rbrakk> \<Longrightarrow> P wp\<^sub>R false is RC"
+  by (rule RC_intro', simp_all add:  wpR_false_RC1 wpR_false_RR)
+ 
+lemma wpR_RC1: "\<lbrakk> P is RR; Q is RC \<rbrakk> \<Longrightarrow> P wp\<^sub>R Q is RC1"
+  by (rule Healthy_intro, simp add: wpR_def RC1_def rpred closure seqr_assoc RC1_prop RC_implies_RC1)
+    
+lemma wpR_RC [closure]: "\<lbrakk> P is RR; Q is RC \<rbrakk> \<Longrightarrow> P wp\<^sub>R Q is RC"
+  by (rule RC_intro', simp_all add: wpR_RC1 closure)
+    
+lemma R2_comp_def: "R2 = R1 \<circ> R2c"
+  by (auto simp add: R2_R2c_def)
+    
+lemma preR_R2_closed [closure]: "P is SRD \<Longrightarrow> pre\<^sub>R(P) is R2"
+  by (simp add: R2_comp_def Healthy_comp closure)
+    
+lemma ISRD_implies_NSRD [closure]: 
+  assumes "P is ISRD"
+  shows "P is NSRD"
+proof -
+  have 1:"ISRD(P) = ISRD1(RD3(SRD(P)))"
+    by (simp add: ISRD_def NSRD_def SRD_def, metis RD1_RD3_commute RD3_left_subsumes_RD2)
+  also have "... = ISRD1(RD3(P))"
+    by (simp add: assms ISRD_implies_SRD Healthy_if)
+  also have "... = ISRD1 (\<^bold>R\<^sub>s ((\<not>\<^sub>r pre\<^sub>R P) wp\<^sub>R false\<^sub>h \<turnstile> (\<exists> $st\<acute> \<bullet> peri\<^sub>R P) \<diamondop> post\<^sub>R P))"
+    by (simp add: RD3_def, subst SRD_right_unit_tri_lemma, simp_all add: assms ISRD_implies_SRD)
+  also have "... = \<^bold>R\<^sub>s ((\<not>\<^sub>r pre\<^sub>R P) wp\<^sub>R false\<^sub>h \<turnstile> false \<diamondop> post\<^sub>R P)"
+    by (simp add: RHS_tri_design_par ISRD1_def unrest choose_srd_def rpred closure ISRD_implies_SRD assms)
+  also have "... = (... ;; II\<^sub>R)"
+    by (rdes_simp, simp add: RHS_tri_normal_design_composition' closure assms unrest ISRD_implies_SRD wp rpred wpR_false_RC)
+  also have "... is RD3"
+    by (simp add: Healthy_def RD3_def seqr_assoc, simp add: NSRD_right_unit closure)
+  finally show ?thesis
+    by (simp add: SRD_RD3_implies_NSRD Healthy_if assms ISRD_implies_SRD)
+qed
+  
+lemma ISRD_form:
+  assumes "P is ISRD"
+  shows "\<^bold>R\<^sub>s(pre\<^sub>R(P) \<turnstile> false \<diamondop> post\<^sub>R(P)) = P"
+proof -
+  have "P = ISRD1(P)"
+    by (simp add: ISRD_implies_ISRD1 assms Healthy_if)
+  also have "... = ISRD1(\<^bold>R\<^sub>s(pre\<^sub>R(P) \<turnstile> peri\<^sub>R(P) \<diamondop> post\<^sub>R(P)))"
+    by (simp add: SRD_reactive_tri_design ISRD_implies_SRD assms)
+  also have "... = \<^bold>R\<^sub>s(pre\<^sub>R(P) \<turnstile> false \<diamondop> post\<^sub>R(P))"
+    by (simp add: ISRD1_rdes_def closure assms ISRD_implies_NSRD)
+  finally show ?thesis ..
+qed
+    
+lemma ISRD_elim: 
+  "\<lbrakk> P is ISRD; Q(\<^bold>R\<^sub>s (pre\<^sub>R(P) \<turnstile> false \<diamondop> post\<^sub>R(P))) \<rbrakk> \<Longrightarrow> Q(P)"
+  by (simp add: ISRD_form)
+  
 lemma skip_srd_ISRD [closure]: "II\<^sub>R is ISRD"
   by (rule ISRD_intro, simp_all add: rdes closure)
     
 lemma assigns_srd_ISRD [closure]: "\<langle>\<sigma>\<rangle>\<^sub>R is ISRD"
   by (rule ISRD_intro, simp_all add: rdes closure)
+    
+lemma Healthy_intro: "H(P) = P \<Longrightarrow> P is H"
+  by (simp add: Healthy_def)
+  
+lemma RC1_prop: 
+  assumes "P is RC1"
+  shows "(\<not>\<^sub>r P) ;; R1 true = (\<not>\<^sub>r P)"
+proof -
+  have "(\<not>\<^sub>r P) = (\<not>\<^sub>r (RC1 P))"
+    by (simp add: Healthy_if assms)
+  also have "... = (\<not>\<^sub>r P) ;; R1 true"
+    by (simp add: RC1_def rpred closure)
+  finally show ?thesis ..
+qed
+     
+lemma seq_ISRD_closed:
+  assumes "P is ISRD" "Q is ISRD"
+  shows "P ;; Q is ISRD"
+  apply (insert assms)
+  apply (erule ISRD_elim)+
+  apply (simp add: rdes_def closure assms unrest)
+done
     
 end
